{-# OPTIONS --without-K --exact-split --safe --auto-inline #-}

open import universes public

-- \MCU for ğ“¤

variable ğ“¤ ğ“¥ ğ“¦ ğ“£ : Universe

-- \^. for Ì‡
-- \b1 for ğŸ™

data ğŸ™ : ğ“¤â‚€ Ì‡  where
 â‹† : ğŸ™

-- \Pi for Î 
ğŸ™-induction : (A : ğŸ™ â†’ ğ“¤â€ŠÌ‡ ) â†’ A â‹† â†’ (x : ğŸ™) â†’ A x
ğŸ™-induction A a â‹† = a

ğŸ™-recursion : (B : ğ“¤ Ì‡) â†’ B â†’ (ğŸ™ â†’ B)
ğŸ™-recursion B b x = ğŸ™-induction (Î» _ â†’ B) b x

!ğŸ™ : {X : ğ“¤â€ŠÌ‡ } â†’ X â†’ ğŸ™
!ğŸ™ _ = â‹†

data ğŸ˜ : ğ“¤â‚€ Ì‡ where

ğŸ˜-induction : (A : ğŸ˜ â†’ ğ“¤ Ì‡) â†’ (x : ğŸ˜) â†’ A x
ğŸ˜-induction A ()

ğŸ˜-recursion : (A : ğ“¤ Ì‡) â†’ ğŸ˜ â†’ A
ğŸ˜-recursion A a = ğŸ˜-induction (Î» _ â†’ A) a

!ğŸ˜ : (A : ğ“¤ Ì‡) â†’ ğŸ˜ â†’ A
!ğŸ˜ = ğŸ˜-recursion

is-empty : ğ“¤ Ì‡ â†’ ğ“¤ Ì‡
is-empty X = X â†’ ğŸ˜

Â¬ : ğ“¤ Ì‡ â†’ ğ“¤ Ì‡
Â¬ X = X â†’ ğŸ˜

data â„• : ğ“¤â‚€ Ì‡ where
  zero : â„•
  succ : â„• â†’ â„•

{-# BUILTIN NATURAL â„• #-}

â„•-induction : (A : â„• â†’ ğ“¤ Ì‡)
            â†’ A 0
            â†’ ((n : â„•) â†’ A n â†’ A (succ n))
            â†’ (n : â„•) â†’ A n
â„•-induction A aâ‚€ f = h
  where
    h : (n : â„•) â†’ A n
    h zero     = aâ‚€
    h (succ x) = f x (h x)

â„•-recursion : (X : ğ“¤ Ì‡)
            â†’ X
            â†’ (â„• â†’ X â†’ X)
            â†’ â„• â†’ X
â„•-recursion X = â„•-induction (Î» _ â†’ X)

â„•-iteration : (X : ğ“¤ Ì‡)
            â†’ X
            â†’ (X â†’ X)
            â†’ â„• â†’ X
â„•-iteration X x f = â„•-recursion X x (Î» _ x â†’ f x)

module Arithmetic where
  _+_  _Ã—_ : â„• â†’ â„• â†’ â„•

  x + y = h y
   where
    h : â„• â†’ â„•
    h = â„•-iteration â„• x succ

  x Ã— y = h y
   where
    h : â„• â†’ â„•
    h = â„•-iteration â„• 0 (x +_)

  infixl 20 _+_
  infixl 21 _Ã—_

module â„•-order where

  _â‰¤_ _â‰¥_ : â„• â†’ â„• â†’ ğ“¤â‚€ Ì‡
  _â‰¤_ = â„•-iteration (â„• â†’ ğ“¤â‚€ Ì‡) (Î» y â†’ ğŸ™)
                    Î» f â†’ â„•-recursion (ğ“¤â‚€ Ì‡) ğŸ˜ Î» y P â†’ f y

  x â‰¥ y = y â‰¤ x

  _â‰¤'_  : â„• â†’ â„• â†’ ğ“¤â‚€ Ì‡
  0      â‰¤' y      = ğŸ™
  succ x â‰¤' 0      = ğŸ˜
  succ x â‰¤' succ y = x â‰¤ y

  infix 10 _â‰¤'_
  infix 10 _â‰¤_
  infix 10 _â‰¥_

  definition-forward : (x y : â„•) â†’ x â‰¤ y â†’ x â‰¤' y
  definition-forward zero y prop = prop
  definition-forward (succ x) (succ y) prop = prop

  definition-backward : (x y : â„•) â†’ x â‰¤' y â†’ x â‰¤ y
  definition-backward zero y prop = prop
  definition-backward (succ x) (succ y) prop = prop


data _+_ {ğ“¤ ğ“¥} (X : ğ“¤ Ì‡) (Y : ğ“¥ Ì‡) : (ğ“¤ âŠ” ğ“¥) Ì‡ where
  inl : X â†’ X + Y
  inr : Y â†’ X + Y

+-induction : {X : ğ“¤ Ì‡} {Y : ğ“¥ Ì‡} (A : X + Y â†’ ğ“¦ Ì‡)
            â†’ ((x : X) â†’ A (inl x))
            â†’ ((y : Y) â†’ A (inr y))
            â†’ (z : X + Y) â†’ A z
+-induction A f g (inl x) = f x
+-induction A f g (inr y) = g y

+-recursion : {X : ğ“¤ Ì‡} {Y : ğ“¥ Ì‡} {A : ğ“¦ Ì‡} â†’ (X â†’ A) â†’ (Y â†’ A) â†’ X + Y â†’ A
+-recursion {ğ“¤} {ğ“¥} {ğ“¦} {X} {Y} {A} = +-induction (Î» _ â†’ A)

ğŸš : ğ“¤â‚€ Ì‡
ğŸš = ğŸ™ + ğŸ™

pattern â‚€ = inl â‹†
pattern â‚ = inr â‹†

ğŸš-induction : (A : ğŸš â†’ ğ“¤ Ì‡) â†’ A â‚€ â†’ A â‚ â†’ (n : ğŸš) â†’ A n
ğŸš-induction A aâ‚€ aâ‚ = +-induction A
                      (ğŸ™-induction (Î» (x : ğŸ™) â†’ A (inl x)) aâ‚€)
                      (ğŸ™-induction (Î» (y : ğŸ™) â†’ A (inr y)) aâ‚)

record Î£ {ğ“¤ ğ“¥} {X : ğ“¤ Ì‡} (Y : X â†’ ğ“¥ Ì‡) : (ğ“¤ âŠ” ğ“¥)Ì‡ where
  constructor
    _,_
  field
    x : X
    y : Y x

-Î£ : {ğ“¤ ğ“¥ : Universe} (X : ğ“¤ Ì‡) (Y : X â†’ ğ“¥ Ì‡) â†’ ğ“¤ âŠ” ğ“¥ Ì‡
-Î£ X Y = Î£ Y

syntax -Î£ X (Î» x â†’ y) = Î£[ x ] X , y

prâ‚ : {X : ğ“¤ Ì‡} {Y : X â†’ ğ“¥ Ì‡} â†’ Î£ Y â†’ X
prâ‚ (x , y) = x

prâ‚‚ : {X : ğ“¤ Ì‡} {Y : X â†’ ğ“¥ Ì‡} â†’ (x : Î£ Y) â†’ Y (prâ‚ x)
prâ‚‚ (x , y) = y

Î£-induction : {X : ğ“¤ Ì‡} {Y : X â†’ ğ“¥ Ì‡} {A : Î£ Y â†’ ğ“¦ Ì‡ }
            â†’ ((x : X) (y : Y x) â†’ A (x , y))
            â†’ ((x , y) : Î£ Y) â†’ A (x , y)
Î£-induction g (x , y) = g x y

curry : {X : ğ“¤ Ì‡} {Y : X â†’ ğ“¥ Ì‡} {A : Î£ Y â†’ ğ“¦ Ì‡ }
      â†’ (((x , y) : Î£ Y) â†’ A (x , y))
      â†’ ((x : X) (y : Y x) â†’ A (x , y))
curry f x y = f (x , y)

_Ã—_ : ğ“¤ Ì‡ â†’ ğ“¥ Ì‡ â†’ (ğ“¤ âŠ” ğ“¥) Ì‡
X Ã— Y = Î£ Î»(x : X) â†’ Y

âˆ : {X : ğ“¤ Ì‡} (A : X â†’ ğ“¥ Ì‡) â†’ ğ“¤ âŠ” ğ“¥ Ì‡
âˆ {ğ“¤} {ğ“¥} {X} A = (x : X) â†’ A x

-âˆ : {ğ“¤ ğ“¥ : Universe} (X : ğ“¤ Ì‡) (Y : X â†’ ğ“¥ Ì‡) â†’ ğ“¤ âŠ” ğ“¥ Ì‡
-âˆ X Y = âˆ Y

id : {X : ğ“¤ Ì‡} â†’ X â†’ X
id x = x

idâ‹† : (X : ğ“¤ Ì‡) â†’ X â†’ X
idâ‹† X = id

_Â·_ : {X : ğ“¤ Ì‡} {Y : ğ“¥ Ì‡} {Z : Y â†’ ğ“¦ Ì‡}
    â†’ ((y : Y) â†’ Z y)
    â†’ (f : X â†’ Y)
    â†’ (x : X) â†’ Z (f x)
g Â· f = Î» x â†’ g (f x)

domain : {X : ğ“¤ Ì‡} {Y : ğ“¥ Ì‡} â†’ (X â†’ Y) â†’ ğ“¤ Ì‡
domain {ğ“¤} {ğ“¥} {X} {Y} f = X

codomain : {X : ğ“¤ Ì‡} {Y : ğ“¥ Ì‡} â†’ (X â†’ Y) â†’ ğ“¥ Ì‡
codomain {ğ“¤} {ğ“¥} {X} {Y} f = Y

type-of : {X : ğ“¤ Ì‡} â†’ X â†’ ğ“¤ Ì‡
type-of {ğ“¤} {X} x = X

data Id {ğ“¤} (X : ğ“¤ Ì‡) : X â†’ X â†’ ğ“¤ Ì‡ where
  refl : (x : X) â†’ Id X x x

_ï¼_ : {X : ğ“¤ Ì‡ } â†’ X â†’ X â†’ ğ“¤ Ì‡
x ï¼ y = Id _ x y

ğ• : (X : ğ“¤ Ì‡) (A : (x y : X) â†’ x ï¼ y â†’ ğ“¥ Ì‡)
  â†’ ((x : X) â†’ A x x (refl x))
  â†’ (x y : X) (p : x ï¼ y) â†’ A x y p
ğ• X A f x x (refl x) = f x

â„ : (X : ğ“¤ Ì‡) (x : X) (B : (y : X) â†’ x ï¼ y â†’ ğ“¥ Ì‡)
  â†’ B x (refl x)
  â†’ (y : X) â†’ (p : x ï¼ y) â†’ B y p
â„ X x B b x (refl x) = b

â„' : (X : ğ“¤ Ì‡) (x : X) (B : (y : X) â†’ x ï¼ y â†’ ğ“¥ Ì‡)
   â†’ B x (refl x)
   â†’ (y : X) â†’ (p : x ï¼ y) â†’ B y p
â„' X x B b = {!!}

ğ•' : (X : ğ“¤ Ì‡) (A : (x y : X) â†’ x ï¼ y â†’ ğ“¥ Ì‡)
   â†’ ((x : X) â†’ A x x (refl x))
   â†’ (x y : X) (p : x ï¼ y) â†’ A x y p
ğ•' X A f x = â„ X x (A x) (f x)

â„s-agreement :  (X : ğ“¤ Ì‡ ) (x : X) (B : (y : X) â†’ x ï¼ y â†’ ğ“¥ Ì‡ )
             â†’ (b : B x (refl x)) â†’ (y : X) (p : x ï¼ y)
             â†’ â„ X x B b y p ï¼ â„' X x B b y p
â„s-agreement = {!!}

ğ•s-agreement :  (X : ğ“¤ Ì‡ ) (A : (x y : X) â†’ x ï¼ y â†’ ğ“¥ Ì‡ )
                (f : (x : X) â†’ A x x (refl x)) (x y : X) (p : x ï¼ y)
             â†’ ğ• X A f x y p ï¼ ğ•' X A f x y p
ğ•s-agreement X A f x x (refl x) = refl (f x)

module exercises_one where
  open â„•-order

  0+x=x : {x : â„•} â†’ (0 Arithmetic.+ x) ï¼ x
  0+x=x = {!!}

  sucxâ‰¤yâ†’xâ‰¤sucy : (x y : â„•) â†’ (succ x) â‰¤ y â†’ x â‰¤ (succ y)
  sucxâ‰¤yâ†’xâ‰¤sucy = {!!}

  exOne : (x y : â„•) â†’ x â‰¤ y â†’ Î£[ z ] â„• , ((x Arithmetic.+ z) ï¼ y)
  exOne = â„•-induction (Î» x â†’ (y : â„•) â†’ x â‰¤ y â†’ -Î£ â„• (Î» z â†’ (x Arithmetic.+ z) ï¼ y)) (Î» y prop â†’ y , 0+x=x)
      (Î»{ n f â†’
        â„•-induction (Î» z â†’ succ n â‰¤ z â†’ -Î£ â„• (Î» zâ‚ â†’ (succ n Arithmetic.+ zâ‚) ï¼ z))
        (Î» imp â†’ !ğŸ˜ (-Î£ â„• (Î» zâ‚ â†’ (succ n Arithmetic.+ zâ‚) ï¼ 0)) imp)
        (Î» n' f' prop â†’ {!!} )})

  exTwo : {x y : â„•} â†’ (x â‰¤ y) ï¼ (Î£[ z ] â„• , ((x Arithmetic.+ z) ï¼ y))
  exTwo = {!!}


